Update syntax.v

syntax.v
@@ -1,66 +1,23 @@
-(*
-switch
-lambda
-tipuri de variabile
-functii + functii de conversie intre tipuri de date
-clase
-tablouri
-*)
-
-(*Sintaxa cod*)
 Require Import Strings.String.
-Local Open Scope string_scope.
-Local Open Scope list_scope.
 Scheme Equality for string.
-Require Import Coq.ZArith.BinInt.
-Local Open Scope Z_scope.
-
-Inductive ERRint  :=
-| err_int :       ERRint
-| int :       Z    -> ERRint.
-
-Inductive ERRbool :=
-| err_bool :      ERRbool
-| boolean :       bool  -> ERRbool.
-
-Inductive ERRstring :=
-| err_string :    ERRstring
-| str  :          string -> ERRstring.
-
-(* array-ul va fi un fel de lista inlantuita fara operator de indexare *)
-
-Inductive ERRarray :=
-| err_array    : ERRarray
-| int_array    : string -> nat -> (list Z)      -> ERRarray
-| bool_array   : string -> nat -> (list bool)   -> ERRarray
-| string_array : string -> nat -> (list string) -> ERRarray.
-
-Notation "[ ]" := nil (format "[ ]") : list_scope.
-Notation "[ a ]" := (cons a nil) : list_scope. 
-Notation "[ a , b , .. , z ]" := (cons a (cons b .. (cons z nil) ..)) : list_scope. 
-
-Notation "A '[-' N '-]' 'i:=' S ":=(int_array    A N S) (at level 50).
-Notation "A '[-' N '-]' 'b:=' S ":=(bool_array   A N S) (at level 50).
-Notation "A '[-' N '-]' 's:=' S ":=(string_array A N S) (at level 50).
-
-Definition initializer_list := [ 1 , 2, 3].
-
-Definition myarr := "arr" [-10-] i:= initializer_list.
-
-Coercion int:      Z >-> ERRint.
-Coercion boolean:  bool >-> ERRbool.
-Coercion str:      string >-> ERRstring.
 
 
+          (*  types definitions + operations *)
+  
+  (* natural *)
 
 
+Require Import Nat.
 
+Inductive ERRnat  :=
+| err_nat :       ERRnat
+| natural :       nat    -> ERRnat.
 
-
+Coercion natural:  nat >-> ERRnat.
 
 Inductive AExp :=
+| acon: ERRnat -> AExp
 | avar: string -> AExp
-| anum: ERRint -> AExp
 | aplus: AExp  -> AExp -> AExp
 | amin:  AExp  -> AExp -> AExp
 | amul:  AExp  -> AExp -> AExp
@@ -71,309 +28,618 @@ Notation "A a- B" := (amin  A B)(at level 71, left associativity).
 Notation "A a* B" := (amul  A B)(at level 69, left associativity).
 Notation "A a/ B" := (adiv  A B)(at level 69, left associativity).
 Notation "A a% B" := (amod  A B)(at level 68, left associativity).
-Coercion anum: ERRint >-> AExp.
+
+Coercion acon: ERRnat >-> AExp.
 Coercion avar: string >-> AExp. 
+
+
+  (* booleans *)
+
+Inductive ERRbool :=
+| err_bool :      ERRbool
+| boolean :       bool  -> ERRbool.
+
+Coercion boolean:  bool >-> ERRbool.
+
 Inductive BExp :=
-| bconst: ERRbool-> BExp
+| bcon:   ERRbool-> BExp
 | bvar:   string -> BExp
 | bnot:   BExp   -> BExp
 | blt:    AExp   -> AExp -> BExp
 | ble:    AExp   -> AExp -> BExp
-| bgt:    AExp   -> AExp -> BExp
-| bge:    AExp   -> AExp -> BExp
 | beq:    AExp   -> AExp -> BExp
 | band:   BExp   -> BExp -> BExp
 | bor:    BExp   -> BExp -> BExp.
-Notation "A  'b<'  B" := (blt  A B) (at level 80).
-Notation "A  'b<=' B" := (ble  A B) (at level 80).
-Notation "A  'b>'  B" := (bgt  A B) (at level 80).
-Notation "A  'b>=' B" := (bge  A B) (at level 80).
 Notation "b!       A" := (bnot   A) (at level 77, left associativity).
-Notation "A  'b='  B" := (beq  A B) (at level 80).
-Notation "A  'b&&' B" := (band A B) (at level 78, left associativity).
-Notation "A  'b||' B" := (bor  A B) (at level 79, left associativity).
-Coercion bconst: ERRbool >-> BExp.
-Coercion bvar: string >-> BExp.
+Notation "A  b<  B" := (blt  A B) (at level 80).
+Notation "A  b<= B" := (ble  A B) (at level 80).
+Notation "A  b=  B" := (beq  A B) (at level 80).
+Notation "A  b&& B" := (band A B) (at level 78, left associativity).
+Notation "A  b|| B" := (bor  A B) (at level 79, left associativity).
 
-Check true b&& true.
-Check "aa" b< "bb".
-Check true b|| false.
-Check true b|| "var".
-
-Inductive StrExp :=
-| strconst : ERRstring -> StrExp
-| strvar :   string    -> StrExp
-| strcat :   StrExp    -> StrExp -> StrExp
-| strtimes : StrExp    -> nat    -> StrExp.
-Notation "A  's+'  B" := (strcat A B)   (at level 82).
-Notation "A  's*'  n" := (strtimes A n) (at level 81).
-Coercion strconst: ERRstring >-> StrExp.
-(* Coercion strvar:   string    >-> StrExp. *)
-
-Check "Mos" s+ "Craciun".
+Coercion bcon : ERRbool >->  BExp.
+Coercion bvar : string >-> BExp.
 
 
-Inductive ArrExp :=
-| arr_length :          ERRarray -> ArrExp
-| arr_add_nat_item :    ERRarray -> nat        ->  ArrExp
-| arr_add_int_item :    ERRarray -> Z          ->  ArrExp
-| arr_add_bool_item :   ERRarray -> bool       ->  ArrExp
-| arr_add_str_item :    ERRarray -> string     ->  ArrExp
-| arr_del_nat_item:     ERRarray -> nat        ->  ArrExp
-| arr_del_int_item:     ERRarray -> Z          ->  ArrExp
-| arr_del_bool_item:    ERRarray -> bool       ->  ArrExp
-| arr_del_str_item:     ERRarray -> string     ->  ArrExp
-| arr_getitem:          ERRarray -> nat        ->  ArrExp.
-Notation "'@' A"        :=(arr_length          A) (at level 67).
-Notation "A 'n<-'  I"   :=(arr_add_nat_item  A I) (at level 68).
-Notation "A 'i<-'  I"   :=(arr_add_int_item  A I) (at level 68).
-Notation "A 'b<-'  I"   :=(arr_add_bool_item A I) (at level 68).
-Notation "A 's<-'  I"   :=(arr_add_str_item  A I) (at level 68).
-Notation "A 'n<-X' I"   :=(arr_del_nat_item  A I) (at level 66).
-Notation "A 'i<-X' I"   :=(arr_del_int_item  A I) (at level 66).
-Notation "A 'b<-X' I"   :=(arr_del_bool_item A I) (at level 66).
-Notation "A 's<-X' I"   :=(arr_del_str_item  A I) (at level 66).
-Notation "A '[[' N ']]'":=(arr_getitem       A N) (at level 69).
+  (* strings *)
+
+Inductive ERRstring :=
+| err_str :       ERRstring
+| str  :          string -> ERRstring.
+
+Coercion str: string >-> ERRstring.
+
+Inductive SExp :=
+| scon : ERRstring -> SExp
+| svar :   string    -> SExp
+| scat :   SExp    -> SExp -> SExp.
+Notation "A s+ B" := (scat A B) (at level 71).
+
+Coercion svar : string >-> SExp.
 
 
-Check @ myarr.
-Check myarr[[ 3 ]].
-
+(* statements *)
 Inductive Stmt :=
-| declInt_l:      string -> AExp   -> Stmt
-| declBool_l:     string -> BExp   -> Stmt
-| declStr_l:      string -> StrExp -> Stmt
+| declNat:        string -> AExp   -> Stmt
+| declBool:       string -> BExp   -> Stmt
+| declStr:        string -> SExp -> Stmt
 
-| declIntArr_l:   string -> nat    -> Stmt
-| declBoolArr_l:  string -> nat    -> Stmt
-| declStrArr_l:   string -> nat    -> Stmt
+| assignNat:      string -> AExp   -> Stmt
+| assignBool:     string -> BExp   -> Stmt
+| assignStr:      string -> SExp -> Stmt
 
-| assignInt_l:    string -> AExp   -> Stmt
-| assignBool_l:   string -> BExp   -> Stmt
-| assignStr_l:    string -> StrExp -> Stmt
-
-| assiIntArr_l:   ERRarray         -> Stmt
-| assiBoolArr_l:  ERRarray         -> Stmt
-| assiStrArr_l:   ERRarray         -> Stmt
-
+| funDecl:        string -> Stmt   -> Stmt -> Stmt
+| funCall:        string -> Stmt
 
 | sequence:   Stmt   -> Stmt   -> Stmt
+
 | whiledo:    BExp   -> Stmt   -> Stmt
-| fordo:      Stmt   -> BExp   -> Stmt -> Stmt -> Stmt
 
 | ifelse:     BExp   -> Stmt   -> Stmt -> Stmt
 | ifthen:     BExp   -> Stmt   -> Stmt
 
-| switch:     AExp   -> Stmt   -> Stmt
-| case:       AExp   -> Stmt   -> Stmt
+| switch_:     AExp   -> Stmt   -> Stmt
+| case_:       AExp   -> Stmt   -> Stmt
 
 | break:      Stmt
-| continue:   Stmt
-
-| callFun:    string -> list string   -> Stmt
-| callLambda: string -> Stmt   -> Stmt -> Stmt.
-
-Notation "'INTEGER' X <- I"                := (declInt_l X I)       (at level 100).
-Notation "'BOOLEAN' X <- B"                := (declBool_l X B)      (at level 100).
-Notation "'STRING'  X <- S"                := (declStr_l X S)       (at level 100).
-Notation " X int<-  I"                     := (assignInt_l X I)     (at level 100).
-Notation " X bool<- B"                     := (assignBool_l X B)    (at level 100).
-Notation " X str<-  S"                     := (assignStr_l X S)     (at level 100).
-Notation "'INTEGER' X '[-' N '-]' := L"    := (assiIntArr_l X N L)  (at level 100).
-Notation "'BOOL'    X '[-' N '-]' := L"    := (assiBoolArr_l X N L) (at level 100).
-Notation "'STRING'  X '[-' N '-]' := L"    := (assiStrArr_l X N L)  (at level 100).
-Notation "S1 ;; S2"                        := (sequence S1 S2)      (at level 100, right associativity).
-Notation "'while' ( B )  { S }"            := (whiledo B S)         (at level 100).
-Notation "'for' ( S1  B  S2 ) { S }"       := (fordo S1 B S2 S)     (at level 100).
-Notation "'if' ( B ) { S1 } 'else' { S2 }" := (ifelse B S1 S2)      (at level 100).
-Notation "'IF' ( B ) { S }"                := (ifthen B S)          (at level 100).
-Notation "'switch' ( A ) { S }"            := (switch A S)          (at level 100).
-Notation "'case' :: A    S"                := (case A S)            (at level 100).
-Notation "'call' N ( S1 )"                 := (callFun N S1)        (at level 100).
+| void:        Stmt.
+Notation "'NATURAL' X :n= N"                := (declNat  X N)      (at level 90).
+Notation "'BOOLEAN' X :b= B"                := (declBool X B)      (at level 90).
+Notation "'STRING'  X :s= S"                := (declStr  X S)      (at level 90).
+Notation "X <n-  N"                         := (assignNat X N)     (at level 90).
+Notation "X <b-  N"                         := (assignBool X N)    (at level 90).
+Notation "X <s-  N"                         := (assignStr X N)     (at level 90).
+Notation "'function' N # P # '{' S '}'"     := (funDecl N P S)     (at level 91).
+Notation "'CALL' N "                        := (funCall N)         (at level 90).
+Notation "S1 ;; S2"                         := (sequence S1 S2)    (at level 92, right associativity).
+Notation "'while' '[' B ']'  S "            := (whiledo B S)       (at level 89).
+(*ifelse*)
+(*ifthen*)
+(* Notation "'switch' A  '[' S ']'"            := (switch A S)        (at level 90). *)
+(* Notation "'case' '>' A '<' S "              := (case A S)          (at level 90). *)
 
 
 Inductive Result :=
-| subCode :         Stmt      -> Result
-| errUndecl :       Result
-| errAssign :       Result
-| default :         Result
-| intResult :       ERRint    -> Result
+| code :            Stmt      -> Result 
+| undeclared :      Result
+| naturalResult :   ERRnat    -> Result
 | booleanResult :   ERRbool   -> Result
 | stringResult :    ERRstring -> Result.
 
 
-Inductive Program :=
-| seqPrg:        Program -> Program -> Program
-| declMain:      Stmt    -> Program
-| declFun:       string  -> list string  -> Stmt     -> Program
+Definition check_eq_over_types (t1 : Result)(t2 : Result) : bool :=
+  match t1 with
+| code c => match t2 with 
+                   | code c => true
+                   | _ => false
+                   end
+| undeclared => match t2 with 
+                   | undeclared => true
+                   | _ => false
+                   end
+| naturalResult n=> match t2 with 
+                   | naturalResult n=> true
+                   | _ => false
+                   end
+| booleanResult n=> match t2 with 
+                   | booleanResult n=> true
+                   | _ => false
+                   end
+| stringResult n=> match t2 with 
+                   | stringResult n=> true
+                   | _ => false
+                   end
+  end.
 
-| declInt_g:     string  -> AExp   -> Program
-| declBool_g:    string  -> BExp   -> Program
-| declStr_g:     string  -> StrExp -> Program
 
-| declClass:     string  -> Stmt   -> Program.
-Notation "P1 '|' P2"                      := (seqPrg P1 P2)   (at level 100).
-Notation "'MAIN' '{(' S ')}'"       := (declMain S)     (at level 100).
-Notation "'function' N  (( S )) { SS }"   := (declFun N S SS) (at level 100).
-Notation "'GLOBAL' 'INTEGER' X ':=' I" := (declInt_g X I)  (at level 100).
-Notation "'GLOBAL' 'BOOL'    X ':=' I" := (declInt_g X I)  (at level 100).
-Notation "'GLOBAL' 'STRING'  X ':=' I" := (declInt_g X I)  (at level 100).
+(*result for natural*)
+
+Definition aplus_result (x y : Result) : Result :=
+  match x, y with
+    | (naturalResult ( natural x' )) , (naturalResult ( natural y' )) => (naturalResult ( natural ( x' + y' ) )) 
+    | _ , _                                                           =>  naturalResult err_nat
+  end.
+
+Definition amin_result (x y : Result) : Result :=
+  match x, y with
+    | (naturalResult ( natural x' )) , (naturalResult ( natural y' )) => if(Nat.ltb x' y') then (naturalResult err_nat)
+                                                                                           else (naturalResult (natural ( x' - y' )))
+    | _ , _                                                           =>  naturalResult err_nat
+  end.
+
+Definition amul_result (x y : Result) : Result :=
+  match x, y with
+    | (naturalResult ( natural x' )) , (naturalResult ( natural y' )) => (naturalResult ( natural ( x' * y' ) )) 
+    | _ , _                                                           =>  naturalResult err_nat
+  end.
+
+Definition adiv_result (x y : Result) : Result :=
+  match x, y with
+    | (naturalResult ( natural x' )) , (naturalResult ( natural y' )) => match x', y' with
+                                                                         |  x'', 0  => naturalResult (err_nat)
+                                                                         |  x'', y''=> naturalResult ( natural ( x'' / y'' ) )
+                                                                         end
+    | _ , _                                                           =>  naturalResult err_nat
+  end.
+
+Definition amod_result (x y : Result) : Result :=
+  match x, y with
+    | (naturalResult ( natural x' )) , (naturalResult ( natural y' )) => match x', y' with
+                                                                         |  x'', 0  => naturalResult (err_nat)
+                                                                         |  x'', y''=> naturalResult ( natural ( x'' mod y'' ) )
+                                                                         end
+    | _ , _                                                           =>  naturalResult err_nat
+  end.
 
 
-Check 
-  declFun "cmmdc" ( [ "x" , "y" ] )
-  (
-      whiledo ( b! ("x" b= "y" ) )
-      (
-          ifelse ( "x" b> "y" )
-             ("x" int<- "x" a- "y")
 
-             ("y" int<- "y" a- "x")
-      )
-  )
-  |
-  declMain
-  (
-      INTEGER "a" <- 25 ;;
-      INTEGER "b" <- 10 ;;
-      callFun "cmmdc" [ "a" , "b" ]
-  )
+
+
+(*result for booleans*)
+
+Definition bnot_result (x : Result) : Result :=
+  match x with
+    | booleanResult ( boolean true  ) => booleanResult ( boolean false )
+    | booleanResult ( boolean false ) => booleanResult ( boolean true  )
+    | _                               => booleanResult   err_bool
+  end.
+
+Definition blt_result (x y : Result) : Result :=
+  match x, y with
+    | (naturalResult ( natural n1 )) , (naturalResult ( natural n2 )) => if ( n1 <? n2 ) then booleanResult ( boolean true )
+                                                                                        else booleanResult ( boolean false)   
+    | _ , _                                                           =>  booleanResult err_bool
+  end.
+
+Definition ble_result (x y : Result) : Result :=
+  match x, y with
+    | (naturalResult ( natural n1 )) , (naturalResult ( natural n2 )) => if ( n1 <=? n2 ) then booleanResult ( boolean true )
+                                                                                        else booleanResult ( boolean false)   
+    | _ , _                                                           =>  booleanResult err_bool
+  end.
+
+Definition beq_result (x y : Result) : Result :=
+  match x, y with
+    | (naturalResult ( natural n1 )) , (naturalResult ( natural n2 )) => if ( n1 =? n2 ) then booleanResult ( boolean true )
+                                                                                        else booleanResult ( boolean false)   
+    | _ , _                                                           =>  booleanResult err_bool
+  end.
+
+Definition band_result (x y : Result) : Result :=
+  match x, y with
+    | (booleanResult ( boolean true  )) , (booleanResult ( boolean true  )) => booleanResult ( boolean true  )
+    | (booleanResult ( boolean true  )) , (booleanResult ( boolean false )) => booleanResult ( boolean false )
+    | (booleanResult ( boolean false )) , (booleanResult ( boolean true  )) => booleanResult ( boolean false )
+    | (booleanResult ( boolean false )) , (booleanResult ( boolean false )) => booleanResult ( boolean false )  
+    | _ , _                                                                 => booleanResult   err_bool
+  end.
+
+Definition bor_result (x y : Result) : Result :=
+  match x, y with
+    | (booleanResult ( boolean true  )) , (booleanResult ( boolean true  )) => booleanResult ( boolean true  )
+    | (booleanResult ( boolean true  )) , (booleanResult ( boolean false )) => booleanResult ( boolean true  )
+    | (booleanResult ( boolean false )) , (booleanResult ( boolean true  )) => booleanResult ( boolean true  )
+    | (booleanResult ( boolean false )) , (booleanResult ( boolean false )) => booleanResult ( boolean false )  
+    | _ , _                                                                 => booleanResult   err_bool
+  end.
+
+
+(*result for strings*)
+
+Definition scat_result (x y : Result) : Result :=
+  match x, y with
+    | (stringResult ( str s1 )) , (stringResult ( str s2 )) => stringResult ( str ( s1 ++ s2   ) )
+    | _ , _                                                 => stringResult ( err_str )
+  end. 
+
+
+
+(* environment + semantics*)
+
+Definition Env := string -> Result.
+
+Definition env0 : Env := fun x => undeclared.
+
+Definition update (env : Env) (x : string) (v : Result) : Env :=
+fun y=>
+  if ( string_eq_dec y x )  then v
+                            else (env y)
 .
 
 
 
-Inductive Memory :=
-| mem_default : Memory
-| offset      : nat   -> Memory.
+
+Reserved Notation "A =[ S ]=> N" (at level 60).
+Inductive aeval : AExp -> Env -> Result -> Prop :=
+| a_const :   forall n sigma,    
+                acon n =[ sigma ]=> (naturalResult n)
+| a_var :     forall v sigma,    
+                avar v =[ sigma ]=> (sigma v)
+| a_add :     forall a1 a2 i1 i2 sigma n,
+                a1 =[ sigma ]=> i1 ->
+                a2 =[ sigma ]=> i2 ->
+                n = aplus_result i1 i2 -> 
+                (a1 a+ a2) =[ sigma ]=> n
+| a_minus :   forall a1 a2 i1 i2 sigma n,
+                a1 =[ sigma ]=> i1 ->
+                a2 =[ sigma ]=> i2 ->
+                n = amin_result i1 i2 -> 
+                (a1 a- a2) =[ sigma ]=> n
+| a_times :   forall a1 a2 i1 i2 sigma n,
+                a1 =[ sigma ]=> i1 ->
+                a2 =[ sigma ]=> i2 ->
+                n = amul_result i1 i2 -> 
+                (a1 a* a2) =[ sigma ]=> n
+| a_divide :  forall a1 a2 i1 i2 sigma n,
+                a1 =[ sigma ]=> i1 ->
+                a2 =[ sigma ]=> i2 ->
+                n = adiv_result i1 i2 -> 
+                (a1 a/ a2) =[ sigma ]=> n
+| a_modullo : forall a1 a2 i1 i2 sigma n,
+                a1 =[ sigma ]=> i1 ->
+                a2 =[ sigma ]=> i2 ->
+                n = amod_result i1 i2 -> 
+                (a1 a% a2) =[ sigma ]=> n
+where "a =[ sigma ]=> n" := (aeval a sigma n).
+
+Reserved Notation "B ={ E }=> B'" (at level 60).
+Inductive beval : BExp -> Env -> Result -> Prop :=
+| b_const :   forall b env,    
+                bcon b ={ env }=> booleanResult b
+| b_var :     forall v env,    
+                bvar v ={ env }=> (env v)
+| b_not :     forall b i env n,
+                b ={ env }=> i ->
+                n = bnot_result i -> 
+                (b! b) ={ env }=> n
+| b_ltb :   forall a1 a2 i1 i2 env n,
+                a1 =[ env ]=> i1 ->
+                a2 =[ env ]=> i2 ->
+                n = blt_result i1 i2 -> 
+                (a1 b< a2) ={ env }=> n
+| b_lte :   forall a1 a2 i1 i2 env n,
+                a1 =[ env ]=> i1 ->
+                a2 =[ env ]=> i2 ->
+                n = ble_result i1 i2 -> 
+                (a1 b<= a2) ={ env }=> n
+| b_eqb :  forall a1 a2 i1 i2 env n,
+                a1 =[ env ]=> i1 ->
+                a2 =[ env ]=> i2 ->
+                n = beq_result i1 i2 -> 
+                (a1 b= a2) ={ env }=> n
+| b_and : forall b1 b2 i1 i2 env n,
+                b1 ={ env }=> i1 ->
+                b2 ={ env }=> i2 ->
+                n = band_result i1 i2 -> 
+                (b1 b&& b2) ={ env }=> n
+| b_or : forall b1 b2 i1 i2 env n,
+                b1 ={ env }=> i1 ->
+                b2 ={ env }=> i2 ->
+                n = bor_result i1 i2 -> 
+                (b1 b|| b2) ={ env }=> n
+where "B ={ env }=> B'" := (beval B env B').
+
+Reserved Notation "S =# V #=> S'" (at level 60).
+Inductive seval : SExp -> Env -> Result -> Prop :=
+| s_const :   forall s env,    
+                scon s =# env #=> stringResult s
+| s_var :     forall v env,    
+                svar v =# env #=> (env v)
+| s_cat :     forall s1 s2 i1 i2 env n,
+                s1 =# env #=> i1 ->
+                s2 =# env #=> i2 ->
+                n = scat_result i1 i2 -> 
+                (s1 s+ s2) =# env #=> n
+where "M =# S #=> N'" := (seval M S N').
 
 
-Definition EnvMem := string -> Memory.
-Definition MemLayer := Memory -> Values.
-Definition Stack := list EnvMem.
-Inductive Config :=
-  | config : nat -> EnvMem -> MemLayer -> Stack -> Config.
-Inductive coada ( tip : Set) : Set :=
-| nill : coada tip
-| elem : tip -> coada tip -> coada tip.
+Scheme Equality for Result.
+
+
+Reserved Notation "S1 -! E !-> S2" (at level 70).
+Inductive eval : Stmt -> Env -> Env -> Prop := 
+| e_declNat :   forall x i n sigma sigma',
+                  ( Result_beq undeclared (sigma x) ) = true ->
+                  n =[ sigma ]=> (naturalResult i)             ->
+                  sigma' = (update sigma x (naturalResult i))  ->
+                  ( NATURAL x :n= n ) -! sigma !-> sigma'
+| e_declBool :  forall x i n sigma sigma',
+                  ( Result_beq undeclared (sigma x) ) = true ->
+                  n ={ sigma }=> (booleanResult i)             ->
+                  sigma' = (update sigma x (booleanResult i))  ->
+                  ( BOOLEAN x :b= n ) -! sigma !-> sigma'
+| e_declStr :   forall x i n sigma sigma',
+                  ( Result_beq undeclared (sigma x) ) = true ->
+                  n =# sigma #=> (stringResult i)              ->
+                  sigma' = (update sigma x (stringResult i))  ->
+                  ( STRING x :s= n ) -! sigma !-> sigma'
+
+| e_assignNat : forall x i a sigma sigma',
+                  ( Result_beq undeclared (sigma x) ) = false->
+                  a =[ sigma ]=> (naturalResult i)             ->
+                  sigma' = (update sigma x (naturalResult i))  ->
+                  ( x <n- a ) -! sigma !-> sigma'      
+| e_assignBool :forall x i a sigma sigma',
+                  ( Result_beq undeclared (sigma x) ) = false->
+                  a =[ sigma ]=> (booleanResult i)             ->
+                  sigma' = (update sigma x (booleanResult i))  ->
+                  ( x <n- a ) -! sigma !-> sigma'
+| e_assignStr : forall x i a sigma sigma',
+                  ( Result_beq undeclared (sigma x) ) = false->
+                  a =[ sigma ]=> (stringResult i)             ->
+                  sigma' = (update sigma x (stringResult i))   ->
+                  ( x <n- a ) -! sigma !-> sigma'
+
+| e_funDecl :   forall s P stmt sigma sigma',
+                  P = void ->
+                  (Result_beq undeclared (sigma s)) = true     ->
+                  sigma' = (update sigma s (code stmt))        -> 
+                  funDecl s P stmt -! sigma !-> sigma' 
+| e_funCall :   forall save s sigma sigma',
+                  (Result_beq undeclared (sigma save)) = false ->
+                  sigma save = (code s)                        -> 
+                  s -! sigma !-> sigma'                        ->
+                  funCall save -! sigma !-> sigma'
+
+| e_sequence :  forall s1 s2 sigma sigma1 sigma2,
+                  s1 -! sigma  !-> sigma1                      ->
+                  s2 -! sigma1 !-> sigma2                      ->
+                  (s1 ;; s2) -! sigma !-> sigma2
+
+
+| e_whilefalse: forall b s sigma,
+                  b ={ sigma }=> booleanResult false           ->
+                  (whiledo b s)-! sigma !-> sigma  
+| e_whiletrue:  forall b s sigma sigma',
+                  b ={ sigma }=> booleanResult true            ->
+                  ( s ;; whiledo b s)-! sigma !-> sigma'       ->
+                  (whiledo b s)-! sigma !-> sigma'
+| e_whilebreak: forall b s s1 s2 sigma sigma',
+                  b  ={ sigma }=> booleanResult true           ->
+                  s  = (s1 ;; break ;; s2)                     ->
+                  s1 -! sigma !-> sigma'                       ->
+                  whiledo b s -! sigma !-> sigma'
+
+|e_switch_seq_false : forall a i a1 i1 sigma sigma' s s1 s2,
+                  a =[ sigma ]=> i                             ->
+                  s = ((case_ (a1) (s1)) ;; s2)                 ->
+                  a1 =[ sigma ]=> i1                           ->
+                  false = Result_beq i i1                      ->
+                  (switch_ a s2)  -! sigma !-> sigma'           ->
+                  (switch_ a s )  -! sigma !-> sigma'
+| e_switch_seq_true : forall a i a1 i1 sigma sigma' sigma'' s s1 s2,
+                  a =[ sigma ]=> i                             ->
+                  s = ((case_ a1 s1) ;; s2)                     ->
+                  a1 =[ sigma ]=> i1                           ->
+                  i = i1                                       -> 
+                  s1 -! sigma !-> sigma'                       ->
+                  switch_ a s2 -! sigma' !-> sigma''            ->
+                  switch_ a s  -! sigma  !-> sigma''
+| e_switch_case_true : forall a i a1 i1 sigma sigma' s s1,
+                  a =[ sigma ]=> i                             ->
+                  s = (case_ a1 s1)                             ->
+                  a1 =[ sigma ]=> i1                           ->
+                  i = i1                                       ->
+                  s1 -! sigma !-> sigma'                       ->
+                  switch_ a s -! sigma !-> sigma'
+| e_switch_case_false : forall a i a1 i1 sigma s s1,
+                  a =[ sigma ]=> i ->
+                  s = (case_ a1 s1) ->
+                  a1 =[ sigma ]=> i1 ->
+                  false = Result_beq i i1 ->
+                  switch_ a s -! sigma !-> sigma 
+where "M' -! S' !-> N'" := (eval M' S' N'). 
 
 
 
+Definition function_ex  :=
+function "fun" # void # 
+{
+  NATURAL "var" :n= 5
+} ;;
+CALL "fun";;
+NATURAL "x" :n= 1.
 
-Definition Env := string-> Result.
+Example ex1 : exists ENV, function_ex -! env0 !-> ENV.
+Proof.
+    eexists.
+    unfold function_ex.
+    eapply e_sequence.
+        -eapply e_funDecl.
+            + reflexivity.
+            + simpl. reflexivity.
+            + split.
+        -eapply e_sequence.
+            +eapply e_funCall.
+                -- simpl. reflexivity.
+                -- split. 
+                -- eapply e_declNat.
+                        ++ simpl. reflexivity.
+                        ++ eapply a_const.
+                        ++ split.
+            + eapply e_declNat.
+                -- simpl. reflexivity.
+                -- eapply a_const. 
+                -- split.
+Qed.
+        
 
-(* This function is useful when we need to update the environment based on the state of a variable *)
-Definition equalOverTypes (type1 : Result) (type2 : Result) : bool :=
-  match type1 with
-| errAssign         => match type2 with 
-                    | errAssign => true
-                    | _ => false
-                      end
-| errUndecl         => match type2 with 
-                    | errUndecl => true
-                    | _ => false
-                      end
-| default           => match type2 with 
-                    | default => true
-                    | _ => false
-                      end
-| intResult  x      => match type2 with 
-                    | intResult y => true
-                    | _ => false
-                      end
-| booleanResult x   =>match type2 with 
-                    | booleanResult y => true
-                    | _ => false
-                      end
-| stringResult x    =>match type2 with 
-                    | stringResult y => true
-                    | _ => false
-                      end
+
+Definition switch_ex :=
+NATURAL "x" :n= 5 ;;
+switch_ ( 5 )
+(
+  case_ 5   ( "x" <n- 0 ) ;;
+  case_ 6   ( "x" <n- 1 )
+). 
+
+
+Example ex2 : exists ENV, switch_ex -! env0 !-> ENV.
+Proof.
+    eexists.
+    unfold switch_ex.
+    eapply e_sequence.
+          -eapply e_declNat.
+                + simpl. reflexivity.
+                + eapply a_const.
+                + split.
+          -eapply e_switch_seq_true.
+                +eapply a_const.
+                +intuition.
+                +eapply a_const.
+                +reflexivity.
+                +eapply e_assignNat.
+                    --simpl. reflexivity.
+                    --eapply a_const.
+                    --split.
+                +eapply e_switch_case_false.
+                    --eapply a_const.
+                    --intuition.
+                    --eapply a_const.
+                    --simpl. reflexivity.
+Qed.
+
+
+Definition break_ex :=
+whiledo (1 b< 10)
+(
+  NATURAL "a" :n= 3 ;;
+  NATURAL "x" :n= 5 ;;
+  break
+). 
+
+Inductive BExp1 :=
+| b_True:  BExp1
+| b_False: BExp1
+| b_Var:   string -> BExp1
+| b_Not:   BExp1  -> BExp1
+| b_And:   BExp1  -> BExp1 -> BExp1
+| b_Or:    BExp1  -> BExp1 -> BExp1.
+
+Notation " a &&' b" := (b_And a b ) (at level 50).
+Notation " a ||' b" := (b_Or a b ) (at level 50).
+Notation " !!' b" := (b_Not b ) (at level 50).
+
+Definition EnvB := string ->bool.
+Definition envB := fun x => if string_dec x "var" then false else true.
+
+Require Import Bool.
+
+
+Fixpoint interpret (e : BExp1) (env : EnvB) : bool :=
+  match e with
+  | b_True      => true
+  | b_False     => false
+  | b_Var x     => (env x)
+  | b_Not b     => negb (interpret b env)
+  | b_And b1 b2 => andb (interpret b1 env) (interpret b2 env)
+  | b_Or  b1 b2 => orb  (interpret b1 env) (interpret b2 env)
   end.
 
 
-Definition update (env : Env) ( x: string ) ( v : Values ) : Env :=
-fun y =>
- if(string_beq x y)
-  then 
-      if      ( andb (check_eq_over_types (env y) err_assign ) true )  then v
-      else if ( andb (check_eq_over_types (env y) v)           true )  then v 
-      else if ( andb (check_eq_over_types (env y) default)     true )  then v 
-      else    err_assign
-  else (env y).
+(* Define a stack machine *)
+Inductive Instruction :=
+| push_const :  bool   -> Instruction
+| push_var :    string -> Instruction
+| not_exp :     Instruction
+| and_exp :     Instruction
+| or_exp :      Instruction.
 
+Require Import List.
+Import ListNotations.
 
-Definition aplus_eroareNat (n1 n2 : eroareNat) : eroareNat :=
-  match n1, n2 with
-    | error_nat, _ => error_nat
-    | _, error_nat => error_nat
-    | int v1, int v2 =>  (v1 + v2)
+Definition Stack := list bool.
+Definition run_instruction (i : Instruction)
+         (env : EnvB) (stack : Stack) : Stack :=
+  match i with
+  | push_const c => (c :: stack)
+  | push_var x   => ((env x) :: stack)
+  | not_exp      => match stack with
+                 | n1 :: stack' => ( negb n1) :: stack'
+                 | _ => stack
+                  end  
+  | and_exp      => match stack with
+                 | n1 :: n2 :: stack' => ( andb n1 n2) :: stack'
+                 | _ => stack
+                 end 
+  | or_exp       => match stack with
+                 | n1 :: n2 :: stack' => ( orb n1 n2) :: stack'
+                 | _ => stack
+                 end
   end.
 
-Definition amin_eroareNat  (n1 n2 : eroareNat) : eroareNat :=
-  match n1, n2 with
-    | error_nat, _ => error_nat
-    | _, error_nat => error_nat
-    | int n1, int n2 => if Nat.ltb n1 n2
-                        then error_nat
-                        else  (n1 - n2)
+
+Fixpoint run_instructions (is' : list Instruction)
+         (env : EnvB) (stack : Stack) : Stack :=
+  match is' with
+  | [] => stack
+  | i :: is'' => run_instructions is'' env (run_instruction i env stack)
   end.
 
-Definition amul_eroareNat (n1 n2 : eroareNat) : eroareNat :=
-  match n1, n2 with
-    | error_nat, _ => error_nat
-    | _, error_nat => error_nat
-    | num v1, num v2 =>  (v1 * v2)
-    end.
 
-Definition adiv_eroareNat (n1 n2 : eroareNat) : eroareNat :=
-  match n1, n2 with
-    | error_nat, _ => error_nat
-    | _, error_nat => error_nat
-    | _, num 0 => error_nat
-    | num v1, num v2 =>  (Nat.div v1 v2)
-    end.
+Fixpoint compile (e : BExp1) : list Instruction :=
+  match e with
+  | b_True  => [push_const true]
+  | b_False => [push_const false]
+  | b_Var x => [push_var x]
+  | b_Not x => (compile x ) ++ [not_exp]
+  | b_And e1 e2 => (compile e1) ++ (compile e2) ++ [and_exp]
+  | b_Or e1 e2 => (compile e1) ++ (compile e2) ++ [or_exp]
+  end.
 
-Definition amod_eroareNat (n1 n2 : eroareNat) : eroareNat :=
-  match n1, n2 with
-    | error_nat, _ => error_nat
-    | _, error_nat => error_nat
-    | _, num 0 => error_nat
-    | num v1, num v2 => (v1 - v2 * (Nat.div v1 v2))
-    end.
+Lemma soundness_helper :
+  forall e env stack is',
+    run_instructions (compile e ++ is') env stack =
+    run_instructions is' env ((interpret e env) :: stack).
+Proof.
+  induction e; intros; simpl; trivial.
+  - rewrite <- app_assoc.
+    rewrite IHe. simpl. reflexivity.
+  - rewrite <- app_assoc.
+    rewrite <- app_assoc.
+    rewrite IHe1.
+    rewrite IHe2.
+    simpl.
+    rewrite andb_comm.
+    reflexivity.
+  - rewrite <- app_assoc.
+    rewrite <- app_assoc.
+    rewrite IHe1.
+    rewrite IHe2.
+    simpl.
+    rewrite orb_comm.
+    reflexivity.
+Qed.
 
-
-Inductive typeOfMemory :=
-  | tOM_default : typeOfMemory
-  | offset :  nat -> typeOfMemory. (* contor pentru zona de memorie *)
-
-
-Scheme Equality for Mem.
-
-
-Inductive DataType :=
-| unsigned:  DataType
-| boolean:  DataType.
-
-Inductive Program :=
-| p_assignment: Program
-| p_function:   Program
-| p_sequence:   Program -> Program -> Program.
-
-Inductive Config :=
-| 
-
-(*
-Configuratie 
-    <
-     cod       
-     env       
-     memorie   
-     stack     
-    >
-*)
-
-
-Definition Stack := list Env.
-
+Theorem soundness :
+  forall e env,
+    run_instructions (compile e) env [] =
+    [interpret e env].
+Proof.
+  intros.
+  rewrite <- app_nil_r with (l := (compile e)).
+  rewrite soundness_helper.
+  simpl. trivial.
+Qed.
 
 
